coq/tmp_check_le.v
@@ -1,0 +1,4 @@
+From Coq Require Import Arith.
+Goal True.
+  Check le_0_n.
+Abort.
