coq/tmp_check_power.v
@@ -1,0 +1,5 @@
+From Coq Require Import Arith.
+
+Goal True.
+  Check Nat.pow_succ_r.
+Abort.
